crefine: proof updates for Gamma parameterisation
- use kernel_all_global_addresses base locale for constants -- these are
  not modified by kernel_all_substitute and the base version is the most
  stable name.

- assume `cpuNum = 0` in Machine_C for current unicore proof;
  use explicit cpuNum assumption in the one lemma before Machine_C that
  depends on cpuNum.

- adjust theory imports + locale names and parameters as needed

Signed-off-by: Gerwin Klein <gerwin.klein@proofcraft.systems>

proof/crefine/ARM/SyscallArgs_C.thy
@@ -14,8 +14,8 @@ begin
 
 (*FIXME: arch-split: C kernel names hidden by Haskell names *)
 context kernel_m begin
-abbreviation "msgRegistersC \<equiv> kernel_all_substitute.msgRegisters"
-lemmas msgRegistersC_def = kernel_all_substitute.msgRegisters_def
+abbreviation "msgRegistersC \<equiv> kernel_all_global_addresses.msgRegisters"
+lemmas msgRegistersC_def = kernel_all_global_addresses.msgRegisters_def
 end
 
 context begin interpretation Arch . (*FIXME: arch-split*)
