proof/crefine/AARCH64/VSpace_C.thy
@@ -327,7 +327,7 @@ lemma addrFromKPPtr_spec:
    \<lbrace>\<acute>ret__unsigned_long = addrFromKPPtr (ptr_val (pptr_' s))\<rbrace>"
   apply vcg
   apply (simp add: addrFromKPPtr_def kernelELFBaseOffset_def kernelELFPAddrBase_def
-                   kernelELFBase_def pptrBase_def mask_def)
+                   kernelELFBase_def pptrBase_def mask_def cpu_0)
   done
 
 (* FIXME: move *)
@@ -1576,8 +1576,8 @@ lemma setRegister_ccorres:
 
 lemma msgRegisters_ccorres:
   "n < unat n_msgRegisters \<Longrightarrow>
-  register_from_H (AARCH64_H.msgRegisters ! n) = (index kernel_all_substitute.msgRegisters n)"
-  apply (simp add: kernel_all_substitute.msgRegisters_def msgRegisters_unfold fupdate_def)
+  register_from_H (AARCH64_H.msgRegisters ! n) = (index kernel_all_global_addresses.msgRegisters n)"
+  apply (simp add: kernel_all_global_addresses.msgRegisters_def msgRegisters_unfold fupdate_def)
   apply (simp add: Arrays.update_def n_msgRegisters_def nth_Cons' split: if_split)
   done
 
